Correctness.thy
@@ -67,19 +67,22 @@ proof -
      (FS (flatten_values h\<^sub>c\<^sub>e) (flatten_environment env\<^sub>h) [3 * v\<^sub>h] [])" by (simp add: hempty_def)
   with ECE CS have "chained_state \<Sigma>\<^sub>c\<^sub>e'" by (metis preserve_chained)
   with VCE have VH: "hcontains h\<^sub>c\<^sub>e v\<^sub>h" by simp
-  have "restructurable (US nmem 0 nmem 0 nmem 0 (nmem(0 := 0)) 1 (length ?cd)) ?cd" by simp
-  with EF have "\<exists>\<Sigma>\<^sub>u'. iter (\<tturnstile> ?cd \<leadsto>\<^sub>u) (US nmem 0 nmem 0 nmem 0 (nmem(0 := 0)) 1 (length ?cd)) \<Sigma>\<^sub>u' \<and>
-    FS (flatten_values h\<^sub>c\<^sub>e) (flatten_environment env\<^sub>h) [3 * v\<^sub>h] [] = restructure \<Sigma>\<^sub>u'" by simp_all
-  then obtain \<Sigma>\<^sub>u' where 
-    "iter (\<tturnstile> ?cd \<leadsto>\<^sub>u) (US nmem 0 nmem 0 nmem 0 (nmem(0 := 0)) 1 (length ?cd)) \<Sigma>\<^sub>u' \<and> 
+  have R: "restructurable (US nmem 0 nmem 0 nmem 0 (nmem(0 := 0, 1 := 0)) 2 (length ?cd)) ?cd" 
+    by simp
+  with EF have "\<exists>\<Sigma>\<^sub>u'. 
+    iter (\<tturnstile> ?cd \<leadsto>\<^sub>u) (US nmem 0 nmem 0 nmem 0 (nmem(0 := 0, 1 := 0)) 2 (length ?cd)) \<Sigma>\<^sub>u' \<and>
+      FS (flatten_values h\<^sub>c\<^sub>e) (flatten_environment env\<^sub>h) [3 * v\<^sub>h] [] = restructure \<Sigma>\<^sub>u'" by simp_all
+  then obtain \<Sigma>\<^sub>u' where EU:
+    "iter (\<tturnstile> ?cd \<leadsto>\<^sub>u) (US nmem 0 nmem 0 nmem 0 (nmem(0 := 0, 1 := 0)) 2 (length ?cd)) \<Sigma>\<^sub>u' \<and> 
       FS (flatten_values h\<^sub>c\<^sub>e) (flatten_environment env\<^sub>h) [3 * v\<^sub>h] [] = restructure \<Sigma>\<^sub>u'" by blast
-  moreover then obtain h\<^sub>u hp\<^sub>u e\<^sub>u ep\<^sub>u vs\<^sub>u vp\<^sub>u sh\<^sub>u where VU:
+  moreover with R have R': "restructurable \<Sigma>\<^sub>u' ?cd" by fastforce
+  moreover with EU obtain h\<^sub>u hp\<^sub>u e\<^sub>u ep\<^sub>u vs\<^sub>u vp\<^sub>u sh\<^sub>u where VU:
     "\<Sigma>\<^sub>u' = US h\<^sub>u hp\<^sub>u e\<^sub>u ep\<^sub>u vs\<^sub>u vp\<^sub>u sh\<^sub>u 0 0 \<and> flatten_values h\<^sub>c\<^sub>e = H h\<^sub>u hp\<^sub>u \<and> 
       flatten_environment env\<^sub>h = H e\<^sub>u ep\<^sub>u \<and> listify' vs\<^sub>u vp\<^sub>u = 3 * v\<^sub>h # []" by auto
   moreover hence VSU: "vs\<^sub>u 0 = 3 * v\<^sub>h \<and> vp\<^sub>u = 1" by auto
-  ultimately have "iter (\<tturnstile> ?cd \<leadsto>\<^sub>u) (US nmem 0 nmem 0 nmem 0 (nmem(0 := 0)) 1 (length ?cd)) 
+  ultimately have "iter (\<tturnstile> ?cd \<leadsto>\<^sub>u) (US nmem 0 nmem 0 nmem 0 (nmem(0 := 0, 1 := 0)) 2 (length ?cd)) 
     (US h\<^sub>u hp\<^sub>u e\<^sub>u ep\<^sub>u vs\<^sub>u 1 sh\<^sub>u 0 0)" by simp
-  hence EU: "iter (\<tturnstile> ?cd \<leadsto>\<^sub>u) (US nmem 0 nmem 0 nmem 0 (nmem(0 := 0)) 1 (length ?cd)) 
+  hence EU: "iter (\<tturnstile> ?cd \<leadsto>\<^sub>u) (US nmem 0 nmem 0 nmem 0 (nmem(0 := 0, 1 := 0)) 2 (length ?cd)) 
     (US h\<^sub>u hp\<^sub>u e\<^sub>u ep\<^sub>u vs\<^sub>u 1 sh\<^sub>u 0 0)" by simp
   let ?mem = "(\<lambda>m. case m of Hp \<Rightarrow> h\<^sub>u | Env \<Rightarrow> e\<^sub>u | Val \<Rightarrow> vs\<^sub>u | Stk \<Rightarrow> sh\<^sub>u)"
   let ?rs = "(\<lambda>r. case r of HP \<Rightarrow> hp\<^sub>u | EP \<Rightarrow> ep\<^sub>u | VP \<Rightarrow> Suc 0 | SP \<Rightarrow> 0 | ACC \<Rightarrow> 0 | AC2 \<Rightarrow> 0)"
@@ -90,16 +93,16 @@ proof -
 
   from C T obtain mp where MP: "assemble ?cd = (?cd', mp)" by (cases "assemble ?cd") simp_all
   with EU have "iter (\<tturnstile> ?cd' \<leadsto>\<^sub>a) 
-    (assemble_state mp (US nmem 0 nmem 0 nmem 0 (nmem(0 := 0)) 1 (length ?cd))) 
+    (assemble_state mp (US nmem 0 nmem 0 nmem 0 (nmem(0 := 0, 1 := 0)) 2 (length ?cd))) 
       (assemble_state mp (US h\<^sub>u hp\<^sub>u e\<^sub>u ep\<^sub>u vs\<^sub>u 1 sh\<^sub>u 0 0))" by (metis correcta_iter)
   with MP have "iter (\<tturnstile> ?cd' \<leadsto>\<^sub>a) 
-    (AS (\<lambda>r. if r = SP then Suc 0 else 0) (\<lambda>m. if m = Stk then nmem(0 := 0) else nmem) 
-      (length ?cd')) (AS ?rs ?mem 0)" by simp
+    (AS (\<lambda>r. if r = SP then 2 else 0) (\<lambda>m. if m = Stk then nmem(0 := 0, 1 := 0) else nmem) 
+      (length ?cd')) (AS ?rs ?mem 0)" by simp 
   hence "iter (\<tturnstile> disassemble ?cd' \<leadsto>\<^sub>m) 
-    (disassemble_state (AS (\<lambda>r. if r = SP then Suc 0 else 0) 
-      (\<lambda>m. if m = Stk then nmem(0 := 0) else nmem) (length ?cd'))) 
+    (disassemble_state (AS (\<lambda>r. if r = SP then 2 else 0) 
+      (\<lambda>m. if m = Stk then nmem(0 := 0, 1 := 0) else nmem) (length ?cd'))) 
         (disassemble_state (AS ?rs ?mem 0))" by (metis correctm_iter)
-  with C T have EM: "iter (\<tturnstile> cd \<leadsto>\<^sub>m) (MS ((\<lambda>r. 0)(R4 := 1)) (nmem(3 := 0)) (length cd)) 
+  with C T have EM: "iter (\<tturnstile> cd \<leadsto>\<^sub>m) (MS ((\<lambda>r. 0)(R4 := 2)) (nmem(3 := 0)) (length cd)) 
     (MS (?rs \<circ> inv_register_map) (uncurry ?mem \<circ> unmap_mem) 0)" by auto
   from EC VT have "print_closure c = print_nexpr (erase v\<^sub>t)" by simp
   moreover from EB have "print_bclosure v\<^sub>b = print_tco_closure (tco_val (encode_closure c))" by simp
@@ -115,7 +118,7 @@ proof -
   with PU have PM: "print_mval (uncurry ?mem \<circ> unmap_mem) (4 * (uncurry ?mem \<circ> unmap_mem) 2) = 
     print_nexpr (erase v\<^sub>t)" by (metis print_m)
   have "(?rs \<circ> inv_register_map) R3 = 1 \<and> (?rs \<circ> inv_register_map) R4 = 0" by simp
-  with VN TN EN EM PM show ?thesis by blast
+  with VN TN EN EM PM show ?thesis by blastx
 qed
 
 end
